reviewing interface/implementation merge in StatefulLHAE.fst

src/tls/StatefulLHAE.fst
@@ -4,6 +4,7 @@ module StatefulLHAE
 // Stateful, agile, length-hiding authenticated encryption with additional data
 // (implemented by appending a fragment sequence number to the additional data)
 
+
 open FStar.Heap
 open FStar.HyperHeap
 open FStar.Seq
@@ -32,7 +33,7 @@ type entry (i:id) = (* records that c is an encryption of p with ad *)
   | Entry: c:cipher i -> ad:adata i -> p:dplain i ad c -> entry i
 
 type is_seqn (n:nat) = repr_bytes n <= 8
-type seqn_t = n:nat { repr_bytes n <= 8 } (* NB: REMOVING THIS LINE TRIGGERS A FATAL ERROR WHEN CHECKING writer_seqn *)
+type seqn_t = n:nat { repr_bytes n <= 8 } (* NS: REMOVING THIS LINE TRIGGERS A FATAL ERROR WHEN CHECKING writer_seqn *)
 
 (* typing the log that specifies StatefulLHAE *)
 type st_log_t (r:rid) (i:id) = rref r (s:seq (entry i))
@@ -54,18 +55,18 @@ abstract type state (i:gid) (rw:rw) =
 type reader i = state i Reader
 type writer i = state i Writer
 
-val region: #i:id -> #rw:rw -> state i rw -> Tot (r:rid{r<>root})
+abstract val region: #i:id -> #rw:rw -> state i rw -> Tot (r:rid{r<>root})
 let region #i #rw s = State.region s
 
-val peer_region: #i:id -> #rw:rw -> state i rw -> Tot (r:rid{r<>root})
+abstract val peer_region: #i:id -> #rw:rw -> state i rw -> Tot (r:rid{r<>root})
 let peer_region #i #wr s = s.peer_region
 
 let log_region    = fun (#i:id) (#rw:rw) (s:state i rw) -> if rw=Reader then peer_region s else region s
 
-val log: #i:id -> #rw:rw -> s:state i rw -> Tot (st_log_t (log_region s) i)
+abstract val log: #i:id -> #rw:rw -> s:state i rw -> Tot (st_log_t (log_region s) i)
 let log #i #rw s = s.log
 
-val seqn: #i:id -> #rw:rw -> s:state i rw -> Tot (rref (region s) seqn_t)
+abstract val seqn: #i:id -> #rw:rw -> s:state i rw -> Tot (rref (region s) seqn_t)
 let seqn #i #rw s = s.seqn
 
 abstract opaque type matching (#i:gid) (r:reader i) (w:writer i) =
@@ -119,7 +120,7 @@ assume val unfold_st_inv: #i:id -> r:reader i -> w:writer i -> h:HyperHeap.t ->
        wctr = Seq.length log
        /\ rctr <= wctr )))
 
-val test_gcm_log_inv: h:HyperHeap.t -> i:gid -> r:reader i -> w:writer i{st_inv r w h} -> n:nat -> j:nat -> c:cipher i -> ad:adata i ->
+private val test_gcm_log_inv: h:HyperHeap.t -> i:gid -> r:reader i -> w:writer i{st_inv r w h} -> n:nat -> j:nat -> c:cipher i -> ad:adata i ->
   Lemma (requires (let gcm_log = sel h (AEAD_GCM.State.log w.key) in
 		   j < Seq.length gcm_log
 		   /\ repr_bytes n <= 8
@@ -136,24 +137,23 @@ let refs_in_w (#i:gid) (e:writer i) =
 
 abstract val frame_st_inv: #i:id -> r:reader i -> w:writer i ->  h0:_ -> h1:_ ->
   Lemma (requires st_inv r w h0
-                  /\ equal_on (Set.union (Set.singleton w.region)
-                                        (Set.singleton w.peer_region)) h0 h1)
+                  /\ equal_on (regions_of w) h0 h1)
         (ensures st_inv r w h1)
 let frame_st_inv i r w h0 h1 = ()
 
 abstract val gen: reader_parent:rid -> writer_parent:rid -> i:gid -> ST (both i)
-  (requires (fun h -> True))
+  (requires (fun h -> disjoint reader_parent writer_parent))
   (ensures  (fun h0 (rw:both i) h1 ->
       modifies Set.empty h0 h1
     /\ (let r = fst rw in
        let w = snd rw in
-      fresh_region r.region h0 h1
-    /\ fresh_region w.region h0 h1
-    /\ extends r.region reader_parent
-    /\ extends w.region writer_parent
+      fresh_region (region r) h0 h1
+    /\ fresh_region (region w) h0 h1
+    /\ extends (region r) reader_parent
+    /\ extends (region w) writer_parent
     /\ st_inv r w h1
-    /\ sel h1 w.log = Seq.createEmpty
-    /\ sel h1 r.seqn = 0)))
+    /\ sel h1 (log w) = Seq.createEmpty
+    /\ sel h1 (seqn r) = 0)))
 let gen reader_parent writer_parent i =
   lemma_repr_bytes_values 0;
   ST.recall_region reader_parent;
@@ -186,12 +186,12 @@ abstract val coerce: r0:rid -> p0:rid {disjoint r0 p0} -> role:rw -> i:gid{~(saf
         (requires (fun h -> True))
         (ensures  (fun h0 s h1 ->
           modifies Set.empty h0 h1
-          /\ extends s.region r0
-          /\ extends s.peer_region p0
-          /\ fresh_region s.region h0 h1
-          /\ fresh_region s.peer_region h0 h1
-          /\ sel h1 s.log = Seq.createEmpty
-          /\ sel h1 s.seqn = 0))
+          /\ extends (region s) r0
+          /\ extends (peer_region s) p0
+          /\ fresh_region (region s) h0 h1
+          /\ fresh_region (peer_region s) h0 h1
+          /\ sel h1 (log s) = Seq.createEmpty
+          /\ sel h1 (seqn s) = 0))
 let coerce r0 p0 role i kv iv =
   lemma_repr_bytes_values 0;
   let r = new_region r0 in
@@ -206,27 +206,23 @@ opaque type st_enc_inv (#i:gid) (w:writer i) (h:HyperHeap.t) =
 
 abstract val frame_st_enc_inv: #i:id -> w:writer i ->  h0:_ -> h1:_ ->
   Lemma (requires st_enc_inv w h0
-                  /\ equal_on (Set.union (Set.singleton w.region)
-                                        (Set.singleton w.peer_region)) h0 h1)
+                  /\ equal_on (regions_of w) h0 h1)
         (ensures st_enc_inv w h1)
 let frame_st_enc_inv i w h0 h1 = ()
-
-let refs_in_e (#i:gid) (e:writer i) =
-  !{ as_ref e.log, as_ref e.seqn }
 
 abstract val encrypt: #i:gid -> #ad:adata i
   -> #rg:range{fst rg = snd rg /\ snd rg <= max_TLSPlaintext_fragment_length}
   -> wr:writer i -> f:plain i ad rg -> ST (cipher i)
   (requires (fun h -> 
      st_enc_inv wr h /\ 
-     is_seqn (sel h wr.seqn + 1)))
+     is_seqn (sel h (seqn wr) + 1)))
   (ensures  (fun h0 (c:cipher i) h1 ->
                   st_enc_inv wr h1
-                /\ modifies (Set.singleton wr.region) h0 h1
-                /\ modifies_rref wr.region (refs_in_e wr) h0 h1
-                /\ sel h1 wr.seqn = sel h0 wr.seqn + 1
+                /\ modifies (Set.singleton (region wr)) h0 h1
+                /\ modifies_rref (region wr) (refs_in_w wr) h0 h1
+                /\ sel h1 (seqn wr) = sel h0 (seqn wr) + 1
                 /\ Wider (Range.cipherRangeClass i (length c)) rg
-                /\ sel h1 wr.log = snoc (sel h0 wr.log) (Entry c ad f)))
+                /\ sel h1 (log wr) = snoc (sel h0 (log wr)) (Entry c ad f)))
 let encrypt i ad rg (State _ log seqn key) f =
   let n = !seqn in
   let l= !log in
@@ -241,7 +237,7 @@ opaque type st_dec_inv (#i:gid) (r:reader i) (h:HyperHeap.t) =
 
 abstract val frame_st_dec_inv: #i:id -> rd:reader i -> h0:_ -> h1:_ ->
   Lemma (requires (st_dec_inv rd h0 /\ 
-                   equal_on (Set.union (Set.singleton rd.region) (Set.singleton rd.peer_region)) h0 h1))
+                   equal_on (regions_of rd) h0 h1))
         (ensures st_dec_inv rd h1)
 let frame_st_dec_inv i rd h0 h1 = ()
 
@@ -253,27 +249,28 @@ abstract val decrypt: #i:gid -> #ad:adata i -> rd:reader i
   -> ST (option (dplain i ad c))
   (requires (fun h ->
              (authId i ==> st_dec_inv rd h)
-           /\ is_seqn (sel h rd.seqn + 1)))
-  (ensures (fun h0 (res:option (dplain i ad c)) h1 ->
-               modifies (Set.singleton rd.region) h0 h1
-             /\ modifies_rref rd.region !{as_ref rd.seqn} h0 h1
-             /\ is_seqn (sel h0 rd.seqn + 1)
-             /\ contains_ref rd.log h0
-             /\ Let (sel h0 rd.log)  (fun (log:seq (entry i){log=sel h0 rd.log}) -> 
-               Let (sel h0 rd.seqn) (fun (rctr:nat{rctr=sel h0 rd.seqn}) ->
+           /\ is_seqn (sel h (seqn rd) + 1)))
+  (ensures (fun h0 (res:option (dplain i ad c)) h1 -> 
+               modifies (Set.singleton (region rd)) h0 h1
+             /\ modifies_rref (region rd) !{as_ref (seqn rd)} h0 h1
+             /\ is_seqn (sel h0 (seqn rd) + 1)
+             /\ contains_ref (log rd) h0
+             /\ (Let (sel h0 (log rd))  (fun (lg:seq (entry i){lg=sel h0 (log rd)}) -> 
+                Let (sel h0 (seqn rd)) (fun (rctr:nat{rctr=sel h0 (seqn rd)}) ->
                authId i
-               ==> st_dec_inv rd h0
+               ==> 
+                  st_dec_inv rd h0
                 /\ st_dec_inv rd h1
-                /\ (if is_Some res
+                /\ (if is_Some res 
                    then
-                    (sel h1 rd.seqn = rctr + 1
-                     /\ Some.v res == Entry.p (Seq.index log rctr))
-                   else
-                      Seq.length log = rctr                 // no more ciphers
-                    \/ c <> Entry.c (Seq.index log rctr)      // wrong cipher
-                    \/ ad =!= Entry.ad (Seq.index log rctr)) // wrong ad
+                    (sel h1 (seqn rd) = rctr + 1
+                     /\ Some.v res == Entry.p (Seq.index lg rctr))
+                   else 
+                      Seq.length lg = rctr                 // no more ciphers
+                    \/ c <> Entry.c (Seq.index lg rctr)      // wrong cipher
+                    \/ ad =!= Entry.ad (Seq.index lg rctr)) // wrong ad
              ))
-    ))
+    )))
 
 let decrypt i ad (State _ log seqn key) c = 
   recall log; recall seqn; recall (AEAD_GCM.State.log key);
@@ -290,16 +287,9 @@ let decrypt i ad (State _ log seqn key) c =
 
 (*** TODO ***)
 (* 
-   - stateful.
    - calling gen/coerce adds i to the log of existing keys;
-   - gen can only be called when i is not yet in the log;
-   - we get this precondition from the freshness of the local nonce in i
-
-   - we use a shared, ghost log of encryptions (also subsuming the history)
-   - we encode fatal decryption errors by abstracting over the decryption counter
-
-   - add back in, from decrypt refinement. Last lines
-      /\ sel h1 (StReader.seqn rd) = rctr))))))) //reveal nothing about the seqn if it fails; rendering this key useless
+     gen can only be called when i is not yet in the log;
+     we get this precondition from the freshness of the local nonce in i
 
    - add overflow protection {is_seqn (length s)})
 *)
